Begin conversion process
Signed-off-by: zeramorphic <zeramorphic@proton.me>

ConNF/Counting/SpecSame.lean
@@ -12,6 +12,111 @@ universe u
 namespace ConNF
 
 variable [Params.{u}] [Level] [FOAAssumptions] {β : Λ} [LeLevel β]
-  {S T : Support β} {σ : Spec β} (hS : σ.Specifies S) (hT : σ.Specifies T)
+  {S T : Support β} {hS : S.Strong} {hT : T.Strong}
+  {σ : Spec β} (hσS : σ.Specifies S hS) (hσT : σ.Specifies T hT)
+
+def ConvertAtom (S T : Support β) (A : ExtendedIndex β) (aS aT : Atom) : Prop :=
+  ∃ (i : κ) (hiS : i < S.max) (hiT : i < T.max), S.f i hiS = ⟨A, inl aS⟩ ∧ T.f i hiT = ⟨A, inl aT⟩
+
+def ConvertNearLitter (S T : Support β) (A : ExtendedIndex β) (NS NT : NearLitter) : Prop :=
+  ∃ (i : κ) (hiS : i < S.max) (hiT : i < T.max), S.f i hiS = ⟨A, inr NS⟩ ∧ T.f i hiT = ⟨A, inr NT⟩
+
+theorem convertAtom_subsingleton (A : ExtendedIndex β) (aS aT aT' : Atom)
+    (h : ConvertAtom S T A aS aT) (h' : ConvertAtom S T A aS aT') : aT = aT' := by
+  obtain ⟨i, hiS₁, hiT₁, hiS₂, hiT₂⟩ := h
+  obtain ⟨i', hiS₁', hiT₁', hiS₂', hiT₂'⟩ := h'
+  have h₁ := (hσS.atom_spec i hiS₁ A aS hiS₂).symm.trans (hσT.atom_spec i hiT₁ A aT hiT₂)
+  have h₂ := (hσS.atom_spec i' hiS₁' A aS hiS₂').symm.trans (hσT.atom_spec i' hiT₁' A aT' hiT₂')
+  simp only [SpecCondition.atom.injEq, true_and] at h₁ h₂
+  have := h₁.1.symm.trans h₂.1
+  rw [Set.ext_iff] at this
+  obtain ⟨_, h⟩ := (this i).mp ⟨hiT₁, hiT₂⟩
+  have := hiT₂.symm.trans h
+  cases this
+  rfl
+
+theorem convert_flexible {A : ExtendedIndex β} {NS NT : NearLitter} (h : Flexible A NS.1)
+    {i : κ} (hiS : i < S.max) (hiT : i < T.max)
+    (hiNS : S.f i hiS = ⟨A, inr NS⟩) (hiNT : T.f i hiT = ⟨A, inr NT⟩) : Flexible A NT.1 := by
+  obtain (hN | ⟨⟨hN⟩⟩ | ⟨⟨hN⟩⟩) := flexible_cases' A NT.1
+  · exact hN
+  · have h₁ := hσS.flexible_spec i hiS A NS h hiNS
+    have h₂ := hσT.inflexibleBot_spec i hiT A NT hN hiNT
+    cases h₁.symm.trans h₂
+  · have h₁ := hσS.flexible_spec i hiS A NS h hiNS
+    have h₂ := hσT.inflexibleCoe_spec i hiT A NT hN hiNT
+    cases h₁.symm.trans h₂
+
+theorem convertNearLitter_subsingleton_flexible (A : ExtendedIndex β) (NS NT NT' : NearLitter)
+    (h : ConvertNearLitter S T A NS NT) (h' : ConvertNearLitter S T A NS NT')
+    (hN : Flexible A NS.1) : NT = NT' := by
+  obtain ⟨i, hiS₁, hiT₁, hiS₂, hiT₂⟩ := h
+  obtain ⟨i', hiS₁', hiT₁', hiS₂', hiT₂'⟩ := h'
+  have h₁ := hσS.flexible_spec i hiS₁ A NS hN hiS₂
+  have h₂ := hσS.flexible_spec i' hiS₁' A NS hN hiS₂'
+  have h₃ := hσT.flexible_spec i hiT₁ A NT
+    (convert_flexible hσS hσT hN hiS₁ hiT₁ hiS₂ hiT₂) hiT₂
+  have h₄ := hσT.flexible_spec i' hiT₁' A NT'
+    (convert_flexible hσS hσT  hN hiS₁' hiT₁' hiS₂' hiT₂') hiT₂'
+  have h₅ := h₁.symm.trans h₃
+  have h₆ := h₂.symm.trans h₄
+  simp only [and_true, exists_const, SpecCondition.flexible.injEq, true_and] at h₅ h₆
+  have := h₅.symm.trans h₆
+  rw [Set.ext_iff] at this
+  obtain ⟨_, h⟩ := (this i).mp ⟨hiT₁, hiT₂⟩
+  have := hiT₂.symm.trans h
+  cases this
+  rfl
+
+theorem convert_inflexibleCoe {A : ExtendedIndex β} {NS NT : NearLitter} (P : InflexibleCoePath A)
+    (t : Tangle P.δ) (hNS : NS.1 = fuzz P.hδε t)
+    {i : κ} (hiS : i < S.max) (hiT : i < T.max)
+    (hiNS : S.f i hiS = ⟨A, inr NS⟩) (hiNT : T.f i hiT = ⟨A, inr NT⟩) :
+    ∃ t', NT.1 = fuzz P.hδε t' := by
+  obtain (hN | ⟨⟨hN⟩⟩ | ⟨⟨P', t', hNT⟩⟩) := flexible_cases' A NT.1
+  · have h₁ := hσS.inflexibleCoe_spec i hiS A NS ⟨P, t, hNS⟩ hiNS
+    have h₂ := hσT.flexible_spec i hiT A NT hN hiNT
+    cases h₁.symm.trans h₂
+  · have h₁ := hσS.inflexibleCoe_spec i hiS A NS ⟨P, t, hNS⟩ hiNS
+    have h₂ := hσT.inflexibleBot_spec i hiT A NT hN hiNT
+    cases h₁.symm.trans h₂
+  · have h₁ := hσS.inflexibleCoe_spec i hiS A NS ⟨P, t, hNS⟩ hiNS
+    have h₂ := hσT.inflexibleCoe_spec i hiT A NT ⟨P', t', hNT⟩ hiNT
+    have := h₁.symm.trans h₂
+    simp only [SpecCondition.inflexibleCoe.injEq, heq_eq_eq, true_and] at this
+    cases this.1
+    exact ⟨t', hNT⟩
+
+theorem convertNearLitter_subsingleton (A : ExtendedIndex β) (NS NT NT' : NearLitter)
+    (h : ConvertNearLitter S T A NS NT) (h' : ConvertNearLitter S T A NS NT') : NT = NT' := by
+  obtain (hNS | ⟨⟨hNS⟩⟩ | ⟨⟨P, t, hNS⟩⟩) := flexible_cases' A NS.1
+  · exact convertNearLitter_subsingleton_flexible hσS hσT A NS NT NT' h h' hNS
+  · obtain ⟨i, hiS₁, hiT₁, hiS₂, hiT₂⟩ := h
+    obtain ⟨i', hiS₁', hiT₁', hiS₂', hiT₂'⟩ := h'
+    sorry
+  · obtain ⟨i, hiS₁, hiT₁, hiS₂, hiT₂⟩ := h
+    obtain ⟨i', hiS₁', hiT₁', hiS₂', hiT₂'⟩ := h'
+    have h₁ := hσS.inflexibleCoe_spec i hiS₁ A NS ⟨P, t, hNS⟩ hiS₂
+    have h₂ := hσS.inflexibleCoe_spec i' hiS₁' A NS ⟨P, t, hNS⟩ hiS₂'
+    obtain ⟨u, hNT⟩ := convert_inflexibleCoe hσS hσT P t hNS hiS₁ hiT₁ hiS₂ hiT₂
+    obtain ⟨u', hNT'⟩ := convert_inflexibleCoe hσS hσT P t hNS hiS₁' hiT₁' hiS₂' hiT₂'
+    have h₃ := hσT.inflexibleCoe_spec i hiT₁ A NT ⟨P, u, hNT⟩ hiT₂
+    have h₄ := hσT.inflexibleCoe_spec i' hiT₁' A NT' ⟨P, u', hNT'⟩ hiT₂'
+    have h₅ := h₁.symm.trans h₃
+    have h₆ := h₂.symm.trans h₄
+    clear h₁ h₂ h₃ h₄
+    simp only [SpecCondition.inflexibleCoe.injEq, heq_eq_eq, CodingFunction.code_eq_code_iff,
+      true_and] at h₅ h₆
+    obtain ⟨ρ, h₅, rfl⟩ := h₅
+    obtain ⟨ρ', h₆, rfl⟩ := h₆
+    sorry
+
+def convert (S T : Support β) : StructBehaviour β :=
+  fun A => {
+    atomMap := sorry
+    nearLitterMap := sorry
+    atomMap_dom_small := sorry
+    nearLitterMap_dom_small := sorry
+  }
 
 end ConNF
